wip, new checker interface

pulse/lib/steel/pulse/Pulse.Checker.Common.fst
@@ -79,80 +79,364 @@ let try_frame_pre (#g:env)
     | Inl ok -> ok
     | Inr fail -> T.raise (Framing_failure fail)
 
-#push-options "--z3rlimit_factor 2"
-let replace_equiv_post
-      (r:range)
-      (g:env)
-      (c:comp{stateful_comp c /\ freevars_comp c `Set.subset` FV.vars_of_env g})
-      (ct:Metatheory.comp_typing_u g c)
-      (post_hint:post_hint_opt g)
-  : T.Tac (c1:comp { stateful_comp c1 /\ comp_pre c1 == comp_pre c /\ comp_post_matches_hint c1 post_hint } &
-           st_equiv g c c1)
-  = let g = CP.push_context "replace_equiv_post" r g in
-    let {u=u_c;res=res_c;pre=pre_c;post=post_c} = st_comp_of_comp c in
-    let st_typing = Metatheory.comp_typing_inversion ct in
-    let (| res_c_typing, pre_c_typing, x, post_c_typing |) = Metatheory.st_comp_typing_inversion st_typing in
-    let px = v_as_nv x in
-    let g_post = push_binding g x (fst px) res_c in
-    let post_c_opened = open_term_nv post_c px in
-    match post_hint with
-    | None ->
-      (| c,
-         ST_VPropEquiv
-           g c c x pre_c_typing res_c_typing post_c_typing
-           (VE_Refl _ _)
-           (VE_Refl _ _) |)
-    | Some post ->
-      if not (eq_univ u_c post.u &&
-              eq_tm res_c post.ret_ty)
-      then fail g None 
-            (Printf.sprintf "(%s) Inferred result type does not match annotation.\n\
-                             Expected type %s\n\
-                             Got type %s\n"
-                  (T.range_to_string r)
-                  (P.term_to_string post.ret_ty)
-                  (P.term_to_string res_c))
-      else if (x `Set.mem` freevars post.post)
-      then fail g None "Unexpected variable clash with annotated postcondition"
-      else (
-        let post_opened = open_term_nv post.post px in
-        let post_c_post_eq
-          : vprop_equiv g_post post_c_opened post_opened
-          = Pulse.Checker.Framing.check_vprop_equiv
-              (CP.push_context "check_vprop_equiv" r g_post)
-              post_c_opened
-              post_opened
-              post_c_typing
-        in
-        let st_comp_with_post : st_comp = {
-          u=u_c;
-          res=res_c;
-          pre=pre_c;
-          post=close_term post_opened x
-        } in
-        let c_with_post = c `with_st_comp` st_comp_with_post in
-        assume (close_term post_opened x == post.post);
-        assume (open_term (close_term post_opened x) x == post_opened);
-        (| c_with_post,
-           ST_VPropEquiv
-             g c c_with_post x pre_c_typing res_c_typing post_c_typing
-             (VE_Refl _ _)
-             post_c_post_eq |)
-      )
+let rec vprop_equiv_typing (#g:_) (#t0 #t1:term) (v:vprop_equiv g t0 t1)
+  : GTot ((tot_typing g t0 tm_vprop -> tot_typing g t1 tm_vprop) &
+          (tot_typing g t1 tm_vprop -> tot_typing g t0 tm_vprop))
+        (decreases v)
+  = match v with
+    | VE_Refl _ _ -> (fun x -> x), (fun x -> x)
+
+    | VE_Sym _ _ _ v' -> 
+      let f, g = vprop_equiv_typing v' in
+      g, f
+
+    | VE_Trans g t0 t2 t1 v02 v21 ->
+      let f02, f20 = vprop_equiv_typing v02 in
+      let f21, f12 = vprop_equiv_typing v21 in
+      (fun x -> f21 (f02 x)), 
+      (fun x -> f20 (f12 x))
+
+    | VE_Ctxt g s0 s1 s0' s1' v0 v1 ->
+      let f0, f0' = vprop_equiv_typing v0 in
+      let f1, f1' = vprop_equiv_typing v1 in      
+      let ff (x:tot_typing g (tm_star s0 s1) tm_vprop)
+        : tot_typing g (tm_star s0' s1') tm_vprop
+        = let s0_typing = star_typing_inversion_l x in
+          let s1_typing = star_typing_inversion_r x in
+          let s0'_typing, s1'_typing = f0 s0_typing, f1 s1_typing in
+          star_typing s0'_typing s1'_typing
+      in
+      let gg (x:tot_typing g (tm_star s0' s1') tm_vprop)
+        : tot_typing g (tm_star s0 s1) tm_vprop
+        = let s0'_typing = star_typing_inversion_l x in
+          let s1'_typing = star_typing_inversion_r x in
+          star_typing (f0' s0'_typing) (f1' s1'_typing)        
+      in
+      ff, gg
+
+    | VE_Unit g t ->
+      let fwd (x:tot_typing g (tm_star tm_emp t) tm_vprop)
+        : tot_typing g t tm_vprop
+        = let r = star_typing_inversion_r x in
+          r
+      in
+      let bk (x:tot_typing g t tm_vprop)
+        : tot_typing g (tm_star tm_emp t) tm_vprop
+        = star_typing emp_typing x
+      in
+      fwd, bk
+
+    | VE_Comm g t0 t1 ->
+      let f t0 t1 (x:tot_typing g (tm_star t0 t1) tm_vprop)
+        : tot_typing g (tm_star t1 t0) tm_vprop
+        = let tt0 = star_typing_inversion_l x in
+          let tt1 = star_typing_inversion_r x in
+          star_typing tt1 tt0
+      in
+      f t0 t1, f t1 t0
+
+    | VE_Assoc g t0 t1 t2 ->
+      let fwd (x:tot_typing g (tm_star t0 (tm_star t1 t2)) tm_vprop)
+        : tot_typing g (tm_star (tm_star t0 t1) t2) tm_vprop
+        = let tt0 = star_typing_inversion_l x in
+          let tt12 = star_typing_inversion_r x in
+          let tt1 = star_typing_inversion_l tt12 in
+          let tt2 = star_typing_inversion_r tt12 in
+          star_typing (star_typing tt0 tt1) tt2
+      in
+      let bk (x : tot_typing g (tm_star (tm_star t0 t1) t2) tm_vprop)
+        : tot_typing g (tm_star t0 (tm_star t1 t2)) tm_vprop
+        = let tt01 = star_typing_inversion_l x in
+          let tt2 = star_typing_inversion_r x in
+          let tt0 = star_typing_inversion_l tt01 in
+          let tt1 = star_typing_inversion_r tt01 in
+          star_typing tt0 (star_typing tt1 tt2)
+      in
+      fwd, bk
+   
+    | VE_Ext g t0 t1 token ->
+      let d1, d2 = vprop_eq_typing_inversion g t0 t1 token in
+      (fun _ -> d2),
+      (fun _ -> d1)
+
+
+let k_elab_unit (g:env) (ctxt:term)
+  : continuation_elaborator g ctxt g ctxt
+  = fun p r -> r
+
+let k_elab_trans
+  (#g0:env) (#g1:env { g1 `env_extends` g0 }) (#g2:env { g2 `env_extends` g1 }) (#ctxt0 #ctxt1 #ctxt2:term)
+  (k0:continuation_elaborator g0 ctxt0 g1 ctxt1)
+  (k1:continuation_elaborator g1 ctxt1 g2 ctxt2 { g1 `env_extends` g0})
+   : continuation_elaborator g0 ctxt0 g2 ctxt2
+   = fun post_hint res -> k0 post_hint (k1 post_hint res)
+
+let comp_st_with_post (c:comp_st) (post:term)
+  : c':comp_st { st_comp_of_comp c' == ({ st_comp_of_comp c with post} <: st_comp) } =
+  match c with
+  | C_ST st -> C_ST { st with post }
+  | C_STGhost i st -> C_STGhost i { st with post }
+  | C_STAtomic i st -> C_STAtomic i {st with post}
+
+let ve_unit_r g (p:term) : vprop_equiv g (tm_star p tm_emp) p = 
+  VE_Trans _ _ _ _ (VE_Comm _ _ _) (VE_Unit _ _)
+
+let st_equiv_post (#g:env) (#t:st_term) (#c:comp_st) (d:st_typing g t c)
+                  (post:term { freevars post `Set.subset` freevars (comp_post c)})
+                  (veq: (x:var { fresh_wrt x g (freevars (comp_post c)) } ->
+                         vprop_equiv (push_binding g x ppname_default (comp_res c)) 
+                                     (open_term (comp_post c) x)
+                                     (open_term post x)))
+  : st_typing g t (comp_st_with_post c post)
+  = let c' = comp_st_with_post c post in
+    let (| u_of, pre_typing, x, post_typing |) = Metatheory.(st_comp_typing_inversion (comp_typing_inversion (st_typing_correctness d))) in
+    let veq = veq x in
+    let st_equiv : st_equiv g c c' =
+        ST_VPropEquiv g c c' x pre_typing u_of post_typing (VE_Refl _ _) veq
+    in
+    T_Equiv _ _ _ _ d st_equiv
+
+let simplify_post (#g:env) (#t:st_term) (#c:comp_st) (d:st_typing g t c)
+                  (post:term { comp_post c == tm_star post tm_emp})
+  : st_typing g t (comp_st_with_post c post)
+  = st_equiv_post d post (fun x -> ve_unit_r (push_binding g x ppname_default (comp_res c)) (open_term post x))
+
+let simplify_lemma (c:comp_st) (c':comp_st) (post_hint:option post_hint_t)
+  : Lemma
+    (requires
+        comp_post_matches_hint c post_hint /\
+        comp_res c' == comp_res c /\
+        comp_u c' == comp_u c /\
+        comp_post c' == tm_star (comp_post c) tm_emp)
+    (ensures comp_post_matches_hint (comp_st_with_post c' (comp_post c)) post_hint /\
+             comp_pre (comp_st_with_post c' (comp_post c)) == comp_pre c')
+  = () 
+
+let frame_for_req_in_ctxt (g:env) (ctxt:term) (req:term)
+   = (frame:term &
+      tot_typing g frame tm_vprop &
+      vprop_equiv g (tm_star req frame) ctxt)
+
+let vprop_equiv_typing_bk (#g:env) (#ctxt:_) (ctxt_typing:tot_typing g ctxt tm_vprop)
+                           (#p:_) (d:vprop_equiv g p ctxt)
+  : tot_typing g p tm_vprop 
+  = let _, bk = vprop_equiv_typing d in
+    bk ctxt_typing
+
+
+#push-options "--z3rlimit_factor 4 --ifuel 1 --fuel 0"
+let k_elab_equiv_continutation (#g1:env) (#g2:env { g2 `env_extends` g1 }) (#ctxt #ctxt1 #ctxt2:term)
+  (k:continuation_elaborator g1 ctxt g2 ctxt1)
+  (d:vprop_equiv g2 ctxt1 ctxt2)
+  : continuation_elaborator g1 ctxt g2 ctxt2 =
+  fun post_hint res ->
+  let framing_token : frame_for_req_in_ctxt g2 ctxt1 ctxt2 =
+    let d : vprop_equiv g2 (tm_star ctxt2 tm_emp) ctxt1 = 
+      VE_Trans _ _ _ _ (VE_Comm _ _ _) (VE_Trans _ _ _ _ (VE_Unit _ _) (VE_Sym _ _ _ d)) in
+      (| tm_emp, emp_typing, d |)
+  in
+  let (| st, c, st_d |) = res in
+  if not (stateful_comp c) then k post_hint (| st, c, st_d |)
+  else
+    let (| _, pre_typing, _, _ |) =
+      Metatheory.(st_comp_typing_inversion (comp_typing_inversion (st_typing_correctness st_d))) in
+    let (| c', st_d' |) =
+      Pulse.Checker.Framing.apply_frame (vprop_equiv_typing_bk pre_typing d) st_d framing_token in
+    assert (comp_post c' == tm_star (comp_post c) tm_emp);
+    let st_d' = simplify_post st_d' (comp_post c) in
+    k post_hint (| st, _, st_d' |)
 #pop-options
 
-let repack (#g:env) (#pre:term) (#t:st_term)
-           (x:(c:comp_st { comp_pre c == pre } & st_typing g t c))
-           (post_hint:post_hint_opt g)
-  : T.Tac (checker_result_t g pre post_hint true)
-  = let (| c, d_c |) = x in
-    if stateful_comp c
-    then (
-      FV.st_typing_freevars d_c;
-      let (| c1, c_c1_eq |) = replace_equiv_post t.range g c (Metatheory.st_typing_correctness d_c) post_hint in
-      (| t, c1, T_Equiv _ _ _ _ d_c c_c1_eq |)
+let vprop_equiv_typing_fwd (#g:env) (#ctxt:_) (ctxt_typing:tot_typing g ctxt tm_vprop)
+                           (#p:_) (d:vprop_equiv g ctxt p)
+  : tot_typing g p tm_vprop 
+  = let fwd, _ = vprop_equiv_typing d in
+    fwd ctxt_typing
+
+#push-options "--z3rlimit_factor 4 --ifuel 1 --fuel 0"
+let k_elab_equiv_prefix
+  (#g1:env) (#g2:env { g2 `env_extends` g1 }) (#ctxt1 #ctxt2 #ctxt:term)
+  (k:continuation_elaborator g1 ctxt1 g2 ctxt)
+  (d:vprop_equiv g1 ctxt1 ctxt2)
+  : continuation_elaborator g1 ctxt2 g2 ctxt =
+  fun post_hint res ->
+  let framing_token : frame_for_req_in_ctxt g1 ctxt2 ctxt1 = 
+  let d = VE_Trans _ _ _ _ (VE_Comm _ _ _) (VE_Trans _ _ _ _ (VE_Unit _ _) d) in
+    (| tm_emp, emp_typing, d |)
+  in
+  let res = k post_hint res in
+  let (| st, c, st_d |) = res in
+  if not (stateful_comp c) then (| st, c, st_d |)
+  else let (| _, pre_typing, _, _ |) =
+         Metatheory.(st_comp_typing_inversion (comp_typing_inversion (st_typing_correctness st_d))) in
+       let (| c', st_d' |) =
+         Pulse.Checker.Framing.apply_frame
+           (vprop_equiv_typing_fwd pre_typing d)
+           st_d
+           framing_token in
+        simplify_lemma c c' post_hint;
+        let c''  = comp_st_with_post c' (comp_post c) in
+        let st_d' : st_typing g1 st c'' = simplify_post st_d' (comp_post c) in
+        let res : st_typing_in_ctxt g1 ctxt2 post_hint = (| st, c'', st_d' |) in
+        res
+#pop-options
+
+let k_elab_equiv
+  (#g1:env) (#g2:env { g2 `env_extends` g1 }) (#ctxt1 #ctxt1' #ctxt2 #ctxt2':term)                 
+  (k:continuation_elaborator g1 ctxt1 g2 ctxt2)
+  (d1:vprop_equiv g1 ctxt1 ctxt1')
+  (d2:vprop_equiv g2 ctxt2 ctxt2')
+  : continuation_elaborator g1 ctxt1' g2 ctxt2' =
+  
+  let k : continuation_elaborator g1 ctxt1 g2 ctxt2' =
+    k_elab_equiv_continutation k d2 in
+  let k : continuation_elaborator g1 ctxt1' g2 ctxt2' =
+    k_elab_equiv_prefix k d1 in
+  k
+
+#push-options "--query_stats --fuel 2 --ifuel 2 --split_queries no --z3rlimit_factor 20"
+let continuation_elaborator_with_bind (#g:env) (ctxt:term)
+  (#c1:comp{stateful_comp c1})
+  (#e1:st_term)
+  (e1_typing:st_typing g e1 c1)
+  (ctxt_pre1_typing:tot_typing g (tm_star ctxt (comp_pre c1)) tm_vprop)
+  (x:var { None? (lookup g x) })
+  : T.Tac (continuation_elaborator
+             g (tm_star ctxt (comp_pre c1))
+             (push_binding g x ppname_default (comp_res c1)) (tm_star (open_term (comp_post c1) x) ctxt)) =
+
+  let pre1 = comp_pre c1 in
+  let res1 = comp_res c1 in
+  let post1 = comp_post c1 in
+  let ctxt_typing = star_typing_inversion_l ctxt_pre1_typing in
+  // let p_prop = Metatheory.pure_typing_inversion pure_typing in
+  let v_eq = VE_Comm g ctxt pre1 in
+  let framing_token : frame_for_req_in_ctxt g (tm_star ctxt pre1) pre1 = 
+    (| ctxt, ctxt_typing, VE_Comm g pre1 ctxt  |)
+  in
+  let (| c1, e1_typing |) =
+    Pulse.Checker.Framing.apply_frame ctxt_pre1_typing e1_typing framing_token in
+  let (| u_of_1, pre_typing, _, _ |) =
+    Metatheory.(st_comp_typing_inversion (comp_typing_inversion (st_typing_correctness e1_typing))) in
+  let b = res1 in
+  let g' = push_binding g x ppname_default b in
+  
+  let post1_opened = open_term_nv post1 (v_as_nv x) in
+  let k : continuation_elaborator g (tm_star ctxt pre1) g' (tm_star post1_opened ctxt) =
+    fun post_hint res ->
+    let (| e2, c2, e2_typing |) = res in
+    if not (stateful_comp c2) // || None? post_hint
+    then T.fail "Unexpected non-stateful comp in continuation elaborate"
+    else (
+      let e2_typing : st_typing g' e2 c2 = e2_typing in
+      let e2_closed = close_st_term e2 x in
+      assume (open_st_term e2_closed x == e2);
+      assert (comp_pre c1 == (tm_star ctxt pre1));
+      assert (comp_post c1 == tm_star post1 ctxt);
+      assert (comp_pre c2 == tm_star post1_opened ctxt);
+      assert (open_term (comp_post c1) x == tm_star post1_opened (open_term ctxt x));
+      // ctxt is well-typed, hence ln
+      assume (open_term ctxt x == ctxt);
+      assert (open_term (comp_post c1) x == comp_pre c2);
+      // we closed e2 with x
+      assume (~ (x `Set.mem` freevars_st e2_closed));
+      if x `Set.mem` freevars (comp_post c2)
+      then T.fail "Impossible"
+      else (
+        let t_typing, post_typing =
+          Pulse.Typing.Combinators.bind_res_and_post_typing g (st_comp_of_comp c2) x post_hint in
+        let (| e, c, e_typing |) =
+          Pulse.Typing.Combinators.mk_bind
+            g (tm_star ctxt pre1) 
+            e1 e2_closed c1 c2 (v_as_nv x) e1_typing
+            u_of_1 
+            e2_typing
+            t_typing
+            post_typing
+        in
+        (| e, c, e_typing |)
+      )
     )
-    else (| t, c, d_c |)
+
+  in
+  k
+#pop-options
+
+
+// #push-options "--z3rlimit_factor 2"
+// let replace_equiv_post
+//       (r:range)
+//       (g:env)
+//       (c:comp{stateful_comp c /\ freevars_comp c `Set.subset` FV.vars_of_env g})
+//       (ct:Metatheory.comp_typing_u g c)
+//       (post_hint:post_hint_opt g)
+//   : T.Tac (c1:comp { stateful_comp c1 /\ comp_pre c1 == comp_pre c /\ comp_post_matches_hint c1 post_hint } &
+//            st_equiv g c c1)
+//   = let g = CP.push_context "replace_equiv_post" r g in
+//     let {u=u_c;res=res_c;pre=pre_c;post=post_c} = st_comp_of_comp c in
+//     let st_typing = Metatheory.comp_typing_inversion ct in
+//     let (| res_c_typing, pre_c_typing, x, post_c_typing |) = Metatheory.st_comp_typing_inversion st_typing in
+//     let px = v_as_nv x in
+//     let g_post = push_binding g x (fst px) res_c in
+//     let post_c_opened = open_term_nv post_c px in
+//     match post_hint with
+//     | None ->
+//       (| c,
+//          ST_VPropEquiv
+//            g c c x pre_c_typing res_c_typing post_c_typing
+//            (VE_Refl _ _)
+//            (VE_Refl _ _) |)
+//     | Some post ->
+//       if not (eq_univ u_c post.u &&
+//               eq_tm res_c post.ret_ty)
+//       then fail g None 
+//             (Printf.sprintf "(%s) Inferred result type does not match annotation.\n\
+//                              Expected type %s\n\
+//                              Got type %s\n"
+//                   (T.range_to_string r)
+//                   (P.term_to_string post.ret_ty)
+//                   (P.term_to_string res_c))
+//       else if (x `Set.mem` freevars post.post)
+//       then fail g None "Unexpected variable clash with annotated postcondition"
+//       else (
+//         let post_opened = open_term_nv post.post px in
+//         let post_c_post_eq
+//           : vprop_equiv g_post post_c_opened post_opened
+//           = Pulse.Checker.Framing.check_vprop_equiv
+//               (CP.push_context "check_vprop_equiv" r g_post)
+//               post_c_opened
+//               post_opened
+//               post_c_typing
+//         in
+//         let st_comp_with_post : st_comp = {
+//           u=u_c;
+//           res=res_c;
+//           pre=pre_c;
+//           post=close_term post_opened x
+//         } in
+//         let c_with_post = c `with_st_comp` st_comp_with_post in
+//         assume (close_term post_opened x == post.post);
+//         assume (open_term (close_term post_opened x) x == post_opened);
+//         (| c_with_post,
+//            ST_VPropEquiv
+//              g c c_with_post x pre_c_typing res_c_typing post_c_typing
+//              (VE_Refl _ _)
+//              post_c_post_eq |)
+//       )
+// #pop-options
+
+// let repack (#g:env) (#pre:term) (#t:st_term)
+//            (x:(c:comp_st { comp_pre c == pre } & st_typing g t c))
+//            (post_hint:post_hint_opt g)
+//   : T.Tac (checker_result_t g pre post_hint true)
+//   = let (| c, d_c |) = x in
+//     if stateful_comp c
+//     then (
+//       FV.st_typing_freevars d_c;
+//       let (| c1, c_c1_eq |) = replace_equiv_post t.range g c (Metatheory.st_typing_correctness d_c) post_hint in
+//       (| t, c1, T_Equiv _ _ _ _ d_c c_c1_eq |)
+//     )
+//     else (| t, c, d_c |)
 
 let intro_comp_typing (g:env) 
                       (c:comp_st)
