pulse/lib/steel/pulse/Pulse.Checker.STApp.fst
@@ -33,6 +33,58 @@ let canonicalize_st_typing (#g:env) (#t:st_term) (#c:comp_st) (d:st_typing g t c
     in
     T_Equiv _ _ _ _ d st_eq
 
+let check_st_app
+  (g:env)
+  (t:st_term { Tm_STApp? t.term })
+  (ctxt:vprop)
+  (ctxt_typing:tot_typing g ctxt tm_vprop)
+  (post_hint:post_hint_opt g)
+  : T.Tac (checker_result_t g ctxt post_hint) =
+
+  let g = push_context "st_app" t.range g in
+  let range = t.range in
+  let Tm_STApp { head; arg_qual=qual; arg } = t.term in
+  let (| head, ty_head, dhead |) = check_term g head in
+  debug_log g (fun _ ->
+    T.print (Printf.sprintf "st_app: head = %s, ty_head = %s\n"
+               (P.term_to_string head)
+               (P.term_to_string ty_head)));
+    
+  match is_arrow ty_head with
+  | Some ({binder_ty=formal;binder_ppname=ppname}, bqual, comp_typ) ->
+    is_arrow_tm_arrow ty_head;
+    debug_log g (fun _ ->
+      T.print (Printf.sprintf "st_app, readback comp as %s\n"
+                 (P.comp_to_string comp_typ)));
+    
+    assert (ty_head ==
+            tm_arrow ({binder_ty=formal;binder_ppname=ppname}) bqual comp_typ);
+    
+    if qual = bqual
+    then
+      let (| arg, darg |) = check_term_with_expected_type g arg formal in
+      match comp_typ with
+      | C_ST res
+      | C_STAtomic _ res
+      | C_STGhost _ res ->
+        // This is a real ST application
+        let d : st_typing _ _ (open_comp_with comp_typ arg) =
+          T_STApp g head formal qual comp_typ arg (E dhead) (E darg) in
+        let d = canonicalize_st_typing d in
+        let t = wr (Tm_STApp {head; arg_qual=qual; arg}) in
+        let c = (canon_comp (open_comp_with comp_typ arg)) in
+        let d : st_typing g t c = d in
+
+        admit ()
+       | _ ->
+         fail g (Some t.range) "Expected an effectful application; got a pure term (could it be partially applied by mistake?)"
+     else fail g (Some t.range) (Printf.sprintf "Unexpected qualifier in head type %s of stateful application: head = %s, arg = %s"
+                 (P.term_to_string ty_head)
+                 (P.term_to_string head)
+                 (P.term_to_string arg))
+
+  | _ -> fail g (Some t.range) (Printf.sprintf "Unexpected head type in impure application: %s" (P.term_to_string ty_head))
+
 
 #push-options "--fuel 0 --ifuel 1 --z3rlimit_factor 2"
 let check_stapp
